partway through some changes to Hoare rules for multi step execution

Semantics/Gensyn_Sem_Small.thy
@@ -1,38 +1,52 @@
 theory Gensyn_Sem_Small imports "../Gensyn" "../Gensyn_Descend" "../Mergeable/Mergeable"
+"../Relpath"
                                 
 
 begin
 
-datatype gensyn_small_error =
-  Ok
+datatype gensyn_small_result =
+  Ok childpath
   | BadPath
   | NoFuel
   | Halted (* this means we executed _past_ the end *)
 
+(* new approach to childpath: descend to an arbitrary descendent,
+   or "bubble up" to immediate parent
+*)
+datatype gs_path =
+  GcDown "childpath"
+  | GcUp
 
+(*
 record ('x, 'mstate) g_semr =
   gsr_rel :: "'x \<Rightarrow> 'mstate \<Rightarrow> 'mstate \<Rightarrow> bool"
-  gsr_getpath :: "'mstate \<Rightarrow> childpath \<Rightarrow> bool"
-  gsr_getdir :: "'mstate \<Rightarrow> dir \<Rightarrow> bool"
-
+  gsr_getpath :: "'mstate \<Rightarrow> gs_path \<Rightarrow> bool"
+*)
 record ('x, 'mstate) g_sem =
   gs_sem :: "'x \<Rightarrow> 'mstate \<Rightarrow> 'mstate"
-  gs_getpath :: "'mstate \<Rightarrow> childpath option"
-  gs_getdir :: "'mstate \<Rightarrow> dir"
+  gs_getpath :: "'mstate \<Rightarrow> rel_update"
+(*  gs_getdir :: "'mstate \<Rightarrow> dir" *)
 
+(*
 fun gs_halted :: "('x, 'mstate) g_sem \<Rightarrow> 'mstate \<Rightarrow> bool" where
 "gs_halted gs m = (gs_getpath gs m = None)"
+*)
 
 (* gs_getflag :: "'mstate \<Rightarrow> gensyn_small_flag" *)
-
+(*
+  new change: childpath (root \<rightarrow> this node) as an argument (?)
+  keep the prefix separate
+  how do we determine when we split out?
+*)
+(*
 definition gensyn_sem_small ::
-  "('x, 'mstate) g_semr \<Rightarrow> 
+  "('x, 'mstate) g_semr \<Rightarrow> childpath \<Rightarrow>
    'x gensyn \<Rightarrow> 'mstate \<Rightarrow> 'mstate \<Rightarrow> bool" where
-"gensyn_sem_small gsr syn m m' =
+"gensyn_sem_small gsr path syn m m' =
  (\<exists> cp . gsr_getpath gsr m cp \<and>
  (\<exists> x l . gensyn_get syn cp = Some (G x l) \<and>
   gsr_rel gsr x m m'))"
-
+*)
 (*
 inductive gensyn_sem_small_many ::
   "('x, 'mstate) g_semr \<Rightarrow> 
@@ -51,54 +65,121 @@ definition gensyn_sem_small_many_halt ::
  (\<forall> cp . \<not> gsr_getpath gsr m' cp))"
 *)
 
+fun droplast :: "'a list \<Rightarrow> 'a list option" where
+"droplast [] = None"
+| "droplast [h] = Some []"
+| "droplast (h1#h2#t) =
+   (case droplast (h2#t) of
+    None \<Rightarrow> None
+    | Some p' \<Rightarrow> Some (h1#p'))"
+    
+
+fun gs_pathD :: "gs_path \<Rightarrow> childpath \<Rightarrow> childpath option" where
+"gs_pathD (GcDown p') p = Some (p @ p')"
+| "gs_pathD (GcUp) p = droplast p"
+
+(* 
+  idea: cp never changes in recursive calls.
+  only relative path does.
+
+  and the relative path is only allowed to change by relpath-updates.
+
+  this is supposed to make it so that when we are inside a subtree, 
+  we cannot tell the difference from being at the root.
+
+  however, it seems like in practice maybe sometimes cp will change?
+  the goal was to generalize over this extra cp argument in order to
+  be able to avoid the issues i was having before with hoare triples.
+  however, i am worried that now the triples will be provable but not
+  useful, since we wouldn't be able to find situations where the cp's would
+  be aligned in such a way where they would apply.
+
+  Big question: how and when does the root childpath need to change?
+  How do we keep this from becoming a problem?
+
+  
+*)
 fun gensyn_sem_small_exec ::
   "('x, 'mstate) g_sem \<Rightarrow>
+   childpath \<Rightarrow>
    'x gensyn \<Rightarrow>
    'mstate \<Rightarrow>
-   ('mstate * gensyn_small_error)" where
-"gensyn_sem_small_exec gs syn m =
- (case gs_getpath gs m of
-  None \<Rightarrow> (m, Ok)
-  | Some cp \<Rightarrow> 
-    (case gensyn_get syn cp of
-     None \<Rightarrow> (m, BadPath)
-     | Some (G x _) \<Rightarrow> (gs_sem gs x m, Ok)))"
+   ('mstate * gensyn_small_result)" where
+"gensyn_sem_small_exec gs cp syn m =
+  (case gensyn_get syn cp  of
+      None \<Rightarrow> (m, BadPath)
+      | Some (G x _) \<Rightarrow> 
+      ( let m' = gs_sem gs x m in
+        (case childpath_update cp (gs_getpath gs m') of
+          None \<Rightarrow> (m', Halted)
+          | Some cp' \<Rightarrow> (gs_sem gs x m, Ok cp'))))"
+
+(*
+(case gs_pathD (gs_getpath gs m') cp of
+         None \<Rightarrow> (m', Ok)
+         | Some cp'
+*)
+(*
+  new idea. have local rather than absolute paths
+  so when we get, we get based on a prefix (prefix @ gs_getpath gs m)
+
+  keep prefix in a separate part of state
+*)
+
+(* gs_pathD (gs_getpath gs m) cp *)
+(* idea here: cp + state \<Rightarrow> path that we should be executing this one at.
+*)
+
+(* new approach - 
+   gs_pathD (cp, m') = where to find next instruction
+   cp = where i am executing this instruction
+   
+*)
+
+fun gensyn_sem_small_exec_many ::
+  "('x, 'mstate) g_sem \<Rightarrow>
+   childpath \<Rightarrow>
+   'x gensyn \<Rightarrow>
+   nat \<Rightarrow>
+   'mstate \<Rightarrow>
+   ('mstate * gensyn_small_result)" where
+"gensyn_sem_small_exec_many gs cp syn 0 m =
+  (m, Ok cp)"
+| "gensyn_sem_small_exec_many gs cp syn (Suc n) m =
+  (case gensyn_sem_small_exec gs cp syn m of
+      (m', Ok cp') \<Rightarrow> gensyn_sem_small_exec_many gs cp' syn n m'
+      | (m', x) \<Rightarrow> (m', x))"
 
 (*
 fun gensyn_sem_small_exec_many ::
   "('x, 'mstate) g_sem \<Rightarrow>
+   childpath \<Rightarrow>
    'x gensyn \<Rightarrow>
    nat \<Rightarrow>
    'mstate \<Rightarrow>
    ('mstate * gensyn_small_error)" where
-"gensyn_sem_small_exec_many gs syn 0 m =
-  (case gs_getpath gs m of
-    None \<Rightarrow> (m, Ok)
-    | _ \<Rightarrow>  (m, NoFuel))"
+"gensyn_sem_small_exec_many gs cp syn 0 m =
+  (m, Ok)"
+| "gensyn_sem_small_exec_many gs cp syn (Suc n) m =
+  (case gs_pathD (gs_getpath gs m) cp of
+   None \<Rightarrow> (m, Ok)
+   | Some _ \<Rightarrow>
+    (case gensyn_sem_small_exec gs cp syn m of
+      (m', Ok) \<Rightarrow>
+        (case gs_pathD (gs_getpath gs m') cp of
+         None \<Rightarrow> (m', Ok)
+         | Some cp' \<Rightarrow> gensyn_sem_small_exec_many gs cp' syn n m')
+      | (m', x) \<Rightarrow> (m', x)))"
+*)
+
+(*
 | "gensyn_sem_small_exec_many gs syn (Suc n) m =
    (case gs_getpath gs m of
-    None \<Rightarrow> (m, Halted)
+    None \<Rightarrow> (m, Ok)
     | _ \<Rightarrow> (case gensyn_sem_small_exec gs syn m of
             (m', Ok) \<Rightarrow> gensyn_sem_small_exec_many gs syn n m'
             | (m', f) \<Rightarrow> (m', f)))"
 *)
-
-(* one approach: just don't keep out of fuel flag. *)
-fun gensyn_sem_small_exec_many ::
-  "('x, 'mstate) g_sem \<Rightarrow>
-   'x gensyn \<Rightarrow>
-   nat \<Rightarrow>
-   'mstate \<Rightarrow>
-   ('mstate * gensyn_small_error)" where
-"gensyn_sem_small_exec_many gs syn 0 m =
-  (m, Ok)"
-| "gensyn_sem_small_exec_many gs syn (Suc n) m =
-   (case gs_getpath gs m of
-    None \<Rightarrow> (m, Ok)
-    | _ \<Rightarrow> (case gensyn_sem_small_exec gs syn m of
-            (m', Ok) \<Rightarrow> gensyn_sem_small_exec_many gs syn n m'
-            | (m', f) \<Rightarrow> (m', f)))"
-
 (*
 fun gensyn_sem_small_exec_many ::
   "('x, 'mstate) g_sem \<Rightarrow>
@@ -115,6 +196,7 @@ fun gensyn_sem_small_exec_many ::
 *)
 
 (* TODO: the ordering of checks is weird here and will lead to weird traces. *)
+(*
 fun gensyn_sem_small_exec_trace' ::
   "('x, 'mstate) g_sem \<Rightarrow>
    'x gensyn \<Rightarrow>
@@ -141,6 +223,7 @@ fun gensyn_sem_small_exec_trace ::
 "gensyn_sem_small_exec_trace gs syn n m =
  (case gensyn_sem_small_exec_trace' gs syn n [] m of
   (l, f) \<Rightarrow> (rev l, f))"
+*)
 
 
 end
